## Beweis der Additivität
- $\overline{z + w} = \overline z + \overline w$
###### ls:
-  $\overline{a+ib + c + id} =$
- $= \overline{a+c+i(b+d)}$
- $=(a + c)-i(b+d)$
###### rs:
- $a -ib + c -id =$
- $=(a+c)-i(b+d)$
- 
## Beweis der Multiplikativität:
- $\overline{z \cdot w} = \overline z \cdot \overline w$
###### ls:
-  $\overline{(a+ib)(c+id)}=$
- $=\overline{ac+iad+ibc+i^2bd}$
- $= \overline{ac+i(ad+bc)-bd}=$
- $=\overline{ac-bd+i(ad+bc)}=$
- $=ac-bd-i(ad+bc)$
###### rs:
- $(a-ib)(c-id)=$
- $=ac-iad-ibc+i^2bd=$
- $=ac-bd-i(ad+bc)$
