## Bilinearität
$$\begin{align}
V = \mathbb R^2, \space \space \langle v, w \rangle := v^Tw \\\\
\langle \lambda v + v', w \rangle = (\lambda v + v')^Tw = \big ((\lambda v)^T+(v')^T \big)w = \\
= (\lambda v^T + v'^T)w = \lambda v^Tw + v'^Tw = \\
= \lambda \langle v, w \rangle + \langle v', w\rangle
\end{align}
$$

- äquivalent für $\langle v, \lambda w + w'\rangle$  
## Symmetrie
$$
\begin{align}
V = \mathbb R^2, \langle v, w \rangle = v^Tw \space \space \forall v, w  \in U  \\
\langle v, w \rangle = v^T w = \sum v_i w_i = \sum w_iv_i = w^Tv = \langle w, v\rangle
\end{align}
$$